finished fstar proof

fstar/Storage.fst
@@ -1,26 +1,26 @@
 module Storage
 
-type value a b =
-  | Mtst : value a b
-  | Var : (v : a) -> value a b
-  | Store : (st : value a b) -> (k : b) -> (v : value a b) -> value a b
+type value a =
+  | Mtst : value a
+  | Var : (v : a) -> value a
+  | Store : (st : value a) -> (k : nat) -> (v : value a) -> value a
 
-let rec save #a (#b : eqtype) (st : value a b) (flds : list b)  (v : value a b)
-  : Tot (value a b) (decreases %[flds;st])
+let rec save #a (st : value a) (flds : list nat)  (v : value a)
+  : Tot (value a) (decreases %[flds;st])
   = match st, flds with
     | Mtst, [] -> v
     | Mtst, k :: xs -> Store Mtst k (save Mtst xs v)
     | Var _, _ -> v
-    | Store st x v', [] -> Store st x v'
-    | Store st k v', k' :: ys -> if k = k' then Store st k (save v ys v') else Store (save st (k' :: ys) v') k v
+    | Store st x _, [] -> Store st x v
+    | Store st k v', k' :: ys -> if k = k' then Store st k (save v' ys v) else Store (save st (k' :: ys) v) k v'
 
-let rec select #a (#b : eqtype) (st : value a b) (n : b) : value a b
+let rec select #a (st : value a) (n : nat) : value a
   = match st with
   | Mtst -> Mtst
   | Var st -> Mtst
-  | Store st k v -> if k = n then v else select st k
+  | Store st k v -> if k = n then v else select st n
 
-let rec isStruct #a #b (st : value a b) : bool
+let rec isStruct #a (st : value a) : bool
   = match st with
   | Mtst -> true
   | Var _ -> false
@@ -28,26 +28,10 @@ let rec isStruct #a #b (st : value a b) : bool
   | Store st _ (Var _) -> isStruct st
   | Store st _ (Store v x v2) -> isStruct st && isStruct (Store v x v2)
 
-// let rec isStructInside #a #b (st : value a b) (k : b) (v : value a b) :
-//   Lemma (requires isStruct (Store st k v))
-//     (ensures isStruct st)
-//   = match st with
-//   | Mtst -> _
-//   | Var _ -> _
-//   | Store _ _ _ -> _
-
-
-let rec select_save #a (#b : eqtype) (st : value a b) (k : b) (path : list b) (v : value a b) (k' : b)
+let rec select_save #a (st : value a) (k : nat) (path : list nat) (v : value a) (k' : nat)
   : Lemma (requires isStruct st)
     (ensures select (save st (k :: path) v) k' == (if k = k' then save (select st k') path v else select st k'))
   = match st with
     | Mtst -> _
     | Var _ -> _
-    | Store st' k''' v' ->
-      // isStructInside st' k''' v';
-      select_save st' k path v k;
-      select_save st' k path v k';
-      assume k''' == k;
-      assume k == k';
-      assert ((if k = k' then save (select st k') path v else select st k') == save (select st k') path v);
-      _
+    | Store st' k''' v' -> select_save st' k path v k'
